lean4/Automaton/DFA/ToNFA.lean
@@ -13,15 +13,15 @@ open DFA NFA
 
 namespace ToNFA
 
-variable {σ : Type _} [DecidableEq σ]  {q : Type _} [DecidableEq q]  (td sd : @DFA σ q) (tn sn : @NFA σ q)
+variable {σ : Type _} {q : Type _}  {σs : Finset σ} {qs : Finset q} [DecidableEq σ] [DecidableEq q] (r s td : DFA σs qs)
 
 
 -- to convert into nfa δ, just create singleton for each state
-def dfa_δ_to_nfa_δ : td.qs → td.σs → Finset td.qs := λ q e => {td.δ q e}
+def dfa_δ_to_nfa_δ : qs → σs → Finset qs := λ q e => {td.δ q e}
 
 -- conversion from nfa to dfa
-def dfa_to_nfa : @NFA σ q := by
-  exact {qs := td.qs , init := td.init , fs := td.fs , δ := dfa_δ_to_nfa_δ td : @NFA σ q}
+def dfa_to_nfa : NFA σs qs  := by
+  exact {init := td.init , fs := td.fs , δ := dfa_δ_to_nfa_δ td }
 
 -- the initial state in NFA is same as in the original DFA
 theorem dfa_to_nfa_eq_init : td.init = (dfa_to_nfa td).init := by simp [dfa_to_nfa]
@@ -30,7 +30,7 @@ theorem dfa_to_nfa_eq_init : td.init = (dfa_to_nfa td).init := by simp [dfa_to_n
 theorem dfa_to_nfa_eq_final : td.fs = (dfa_to_nfa td).fs := by simp [dfa_to_nfa]
 
 -- the δ_star function remains the same (but NFA produces singletons)
-theorem dfa_to_nfa_eq_δ_star' (w : word td.σs) : (q : td.qs) → {DFA.δ_star' td q w} = NFA.δ_star' (dfa_to_nfa td) {q} w := by
+theorem dfa_to_nfa_eq_δ_star' (w : word σs) : (q : qs) → {DFA.δ_star' td q w} = NFA.δ_star' (dfa_to_nfa td) {q} w := by
   induction w with
   | nil => intro q; simp [DFA.δ_star,NFA.δ_star]
   | cons a as h => intro q
@@ -38,7 +38,7 @@ theorem dfa_to_nfa_eq_δ_star' (w : word td.σs) : (q : td.qs) → {DFA.δ_star'
                    rw [h]
                    simp [δ_step,dfa_to_nfa,dfa_δ_to_nfa_δ]
 
-theorem dfa_to_nfa_eq_δ_star (w : word td.σs) : {DFA.δ_star td w} = NFA.δ_star (dfa_to_nfa td) w := by
+theorem dfa_to_nfa_eq_δ_star (w : word σs) : {DFA.δ_star td w} = NFA.δ_star (dfa_to_nfa td) w := by
   simp only [DFA.δ_star, NFA.δ_star]
   have h : (dfa_to_nfa td).init = td.init := by simp [dfa_to_nfa]
   rw [h]
