lean4/Automaton/NFA/Basic.lean
@@ -11,39 +11,34 @@ import Mathlib.Data.FinEnum
 
 namespace NFA
 
-structure NFA {σ : Type _} {q : Type _} where
-  σs : Finset σ    -- alphabet
-  qs : Finset q    -- states
+structure NFA (σs : Finset σ) (qs : Finset q) where
   init : qs        -- initial state
   fs : Finset qs   -- accepting states
   δ : qs → σs → Finset qs -- transition function
-  [dq : DecidableEq q]
-  [dσ : DecidableEq σ]
 
-variable {σ : Type _} {q : Type _}  (r s t : @NFA σ q) [DecidableEq σ] [DecidableEq q]
 
-instance : DecidableEq t.σs := by infer_instance
-instance : DecidableEq t.qs := by infer_instance
+variable {σ : Type _} {q : Type _} {σs : Finset σ} {qs : Finset q} (r s t : NFA σs qs) [DecidableEq σ] [DecidableEq q]
+
 
 -- one step in the operation of NFA, consuming one character
 -- take the union of all sets of states reachable from current set of states
 @[simp]
-def δ_step  (q : Finset t.qs) (e : t.σs) : Finset t.qs := q.biUnion (fun n => t.δ n e)
+def δ_step  (q : Finset qs) (e : σs) : Finset qs := q.biUnion (fun n => t.δ n e)
 
 -- δ* function for NFA
 -- returns set of states reached after inputting a word
 @[simp]
-def δ_star' (q : Finset t.qs) : (w : word t.σs) → Finset t.qs
+def δ_star' (q : Finset qs) : (w : word σs) → Finset qs
   | [] => q
   | e :: es => δ_star' (δ_step t q e) es
 
 @[simp]
-def δ_star : (w : word t.σs) → Finset t.qs := δ_star' t {t.init}
+def δ_star : (w : word σs) → Finset qs := δ_star' t {t.init}
 
 -- Whether a word is in the language that the NFA accepts
 @[simp]
-def nfa_accepts (w : word t.σs) : Prop := by
-  have inter : Finset t.qs := (δ_star t w) ∩ t.fs
+def nfa_accepts (w : word σs) : Prop := by
+  have inter : Finset qs := (δ_star t w) ∩ t.fs
   exact inter.Nonempty
 
 -- nfa accepts nil iff init is final
@@ -58,7 +53,7 @@ theorem nfa_accepts_nil_iff_final : nfa_accepts t [] ↔ t.init ∈ t.fs := by
     rw [Finset.singleton_inter_of_mem e]
     exact (Finset.singleton_nonempty t.init)
 
-instance decidableLang (w : word t.σs) : Decidable (nfa_accepts t w) := by
+instance decidableLang (w : word σs) : Decidable (nfa_accepts t w) := by
   dsimp [nfa_accepts]
   apply Finset.decidableNonempty
 
