lean4/Automaton/NFA/ENFA.lean
@@ -11,85 +11,100 @@ open NFA Finset DFA
 
 namespace εNFA
 
-structure εNFA {σ : Type _} {q : Type _} where
-  σs : Finset σ    -- alphabet
-  qs : Finset q    -- states
+structure εNFA (σs : Finset σ) (qs : Finset q) where
   init : qs        -- initial state
   fs : Finset qs   -- accepting states
   δ : qs → Option σs → Finset qs -- transition function
-  [dq : DecidableEq q]
-  [dσ : DecidableEq σ]
-
-variable {σ : Type _} {q : Type _} (r s tn : @εNFA σ q) [DecidableEq σ] [DecidableEq q]
 
 
--- TODO make εclosure definition better
+variable {σ : Type _} {q : Type _} {σs : Finset σ} {qs : Finset q} (r s tn : εNFA σs qs) [DecidableEq σ] [DecidableEq q]
 
-def εclosure_set : Nat → Finset tn.qs → Finset tn.qs
-  | 0 , f => f
-  | n+1 , f => (εclosure_set n f).biUnion (fun s => tn.δ s none) ∪ (εclosure_set n f )
 
-def εclosure : tn.qs → Finset tn.qs := fun q => εclosure_set tn tn.qs.card {q}
+def εclosure (f : Finset qs) : Finset qs := by
+  let newF := f.biUnion (fun q => tn.δ q none) ∪ f
+  if h : f = newF then exact f else exact εclosure newF
+
+termination_by εclosure => qs.card - f.card
+decreasing_by simp at h
+              apply Exists.elim h
+              intro q ex
+              apply Exists.elim ex
+              intro p h
+              have ss : f ⊂ newF := by apply Finset.ssubset_iff_subset_ne.mpr
+                                       apply And.intro
+                                       · apply Finset.subset_union_right
+                                       · intro fe
+                                         have := Finset.right_eq_union_iff_subset.mp fe
+                                         apply h.2
+                                         rw [Finset.biUnion_subset] at this
+                                         apply this
+                                         exact h.1
+              apply Nat.sub_lt_sub_left
+              · have : newF ⊆ qs.attach := by simp [· ⊆· ]
+                have : qs.attach.card = qs.card := by simp
+                rw [←this]
+                apply Finset.card_lt_card
+                apply Finset.ssubset_of_ssubset_of_subset
+                · exact ss
+                · assumption
+              · simp
+                apply Finset.card_lt_card
+                exact ss
+
 
 @[simp]
-def fin_εclosure (f : Finset tn.qs) : Finset tn.qs := f.biUnion (fun q => εclosure tn q)
+def δ_step (q : Finset qs) (e : σs) : Finset qs := (εclosure tn q).biUnion (fun q' => tn.δ q' e)
 
-@[simp]
-def δ_step (q : Finset tn.qs) (e : tn.σs) : Finset tn.qs := (fin_εclosure tn q).biUnion (fun q' => tn.δ q' e)
-
-def δ_star' (q : Finset tn.qs) : (word tn.σs) → Finset tn.qs
-  | [] => fin_εclosure tn q
+def δ_star' (q : Finset qs) : (word σs) → Finset qs
+  | [] => εclosure tn q
   | a :: as => δ_star' (δ_step tn q a) as
 
-def δ_star (w : word tn.σs) : Finset tn.qs := δ_star' tn {tn.init} w
+def δ_star (w : word σs) : Finset qs := δ_star' tn {tn.init} w
 
-def εnfa_accepts (w : word tn.σs) : Prop := (δ_star tn w ∩ tn.fs).Nonempty
+def εnfa_accepts (w : word σs) : Prop := (δ_star tn w ∩ tn.fs).Nonempty
 
 instance : Decidable (εnfa_accepts tn w) := by
   simp only [εnfa_accepts]
   apply Finset.decidableNonempty
 
 @[simp]
-def εnfa_to_nfa_q : Finset (Finset tn.qs) := tn.qs.attach.powerset
+def εnfa_to_nfa_q : Finset (Finset qs) := qs.attach.powerset
 
-theorem all_in_q (qs : Finset tn.qs) : qs ∈ εnfa_to_nfa_q tn := by
-  simp [εnfa_to_nfa_q,finenum_to_finset, · ⊆ ·]
-
-@[simp]
-def εnfa_to_nfa_init : { x // x ∈ εnfa_to_nfa_q tn } := ⟨ εclosure tn tn.init , all_in_q tn (εclosure tn tn.init)⟩
+theorem all_in_q (qs : Finset qs) : qs ∈ εnfa_to_nfa_q := by
+  simp [εnfa_to_nfa_q, · ⊆ ·]
 
 @[simp]
-def εnfa_to_nfa_fs : Finset { x // x ∈ εnfa_to_nfa_q tn } := by
-  have fs := (εnfa_to_nfa_q tn).filter (fun q => (q ∩ tn.fs).Nonempty)
+def εnfa_to_nfa_init : { x // x ∈ @εnfa_to_nfa_q q qs } := ⟨ εclosure tn {tn.init} , all_in_q (εclosure tn {tn.init})⟩
+
+@[simp]
+def εnfa_to_nfa_fs : Finset { x // x ∈ @εnfa_to_nfa_q q qs } := by
+  have fs := εnfa_to_nfa_q.filter (fun q => (q ∩ tn.fs).Nonempty)
   apply fs.biUnion
   intro q
-  exact {⟨q , all_in_q tn q⟩}
+  exact {⟨q , all_in_q q⟩}
 
 @[simp]
-def εnfa_to_nfa_δ :  { x // x ∈ εnfa_to_nfa_q tn } → tn.σs → Finset { x // x ∈ εnfa_to_nfa_q tn } := by
+def εnfa_to_nfa_δ :  { x // x ∈ @εnfa_to_nfa_q q qs } → σs → Finset { x // x ∈ @εnfa_to_nfa_q q qs } := by
   intro q e
-  have := fin_εclosure tn (q.1.biUnion (fun q => tn.δ q e))
-  exact {⟨ this , all_in_q tn this⟩}
+  have := εclosure tn (q.1.biUnion (fun q => tn.δ q e))
+  exact {⟨ this , all_in_q this⟩}
 
 @[simp]
-def εnfa_to_nfa : @NFA σ (Finset {x // x ∈ tn.qs}) :=
-  {qs := εnfa_to_nfa_q tn, σs := tn.σs, init := εnfa_to_nfa_init tn, fs := εnfa_to_nfa_fs tn, δ := εnfa_to_nfa_δ tn}
+def εnfa_to_nfa : NFA σs (@εnfa_to_nfa_q q qs) :=
+  {init := εnfa_to_nfa_init tn, fs := εnfa_to_nfa_fs tn, δ := εnfa_to_nfa_δ tn}
 
-@[simp]
-def εnfa_state_to_nfa_state (q : Finset tn.qs) : Finset ((εnfa_to_nfa tn).qs) := {⟨ q , all_in_q tn q⟩}
-
-theorem δ_star'_eq (w : word tn.σs): (q : Finset tn.qs) → {⟨(εNFA.δ_star' tn q w) , all_in_q tn (εNFA.δ_star' tn q w)⟩} = NFA.δ_star' (εnfa_to_nfa tn) {⟨fin_εclosure tn q , all_in_q tn (fin_εclosure tn q)⟩} w := by
+theorem δ_star'_eq (w : word σs): (q : Finset qs) → {⟨(εNFA.δ_star' tn q w) , all_in_q  (εNFA.δ_star' tn q w)⟩} = NFA.δ_star' (εnfa_to_nfa tn) {⟨εclosure tn q , all_in_q _⟩} w := by
   induction w with
   | nil => simp [δ_star']
   | cons a as s => intro q
                    simp [NFA.δ_star',δ_star',s]
 
-theorem δ_star_eq (w : word tn.σs) : {⟨εNFA.δ_star tn w , all_in_q tn (εNFA.δ_star tn w)⟩ } = NFA.δ_star (εnfa_to_nfa tn) w := by
+theorem δ_star_eq (w : word σs) : {⟨εNFA.δ_star tn w , all_in_q  (εNFA.δ_star tn w)⟩ } = NFA.δ_star (εnfa_to_nfa tn) w := by
   simp only [δ_star]
   rw [δ_star'_eq tn w {tn.init}]
   simp
 
-theorem εnfa_to_nfa_eq (w : word tn.σs) : εnfa_accepts tn w ↔ nfa_accepts (εnfa_to_nfa tn) w := by
+theorem εnfa_to_nfa_eq (w : word σs) : εnfa_accepts tn w ↔ nfa_accepts (εnfa_to_nfa tn) w := by
   simp only [nfa_accepts,εnfa_accepts]
   apply Iff.intro
   · intro a
@@ -102,7 +117,7 @@ theorem εnfa_to_nfa_eq (w : word tn.σs) : εnfa_accepts tn w ↔ nfa_accepts (
     · simp [δ_star]
   . intro a
     rw [←δ_star_eq] at a
-    have := nonempty_inter_singleton_imp_in ⟨δ_star tn w, all_in_q tn (δ_star tn w)⟩ (εnfa_to_nfa tn).fs
+    have := nonempty_inter_singleton_imp_in ⟨δ_star tn w, all_in_q (δ_star tn w)⟩ (εnfa_to_nfa tn).fs
     have := this a
     simp only [δ_star,εnfa_to_nfa,εnfa_to_nfa_fs,Finset.mem_biUnion,Finset.mem_singleton,Finset.mem_filter] at this
     apply Exists.elim this
