lean4/Automaton/NFA/Examples.lean
@@ -2,34 +2,74 @@ import Automaton.NFA.Basic
 import Automaton.DFA.Minimization
 import Automaton.DFA.ToNFA
 import Automaton.NFA.ToDFA
+import Automaton.NFA.ENFA
 
 -- normal automaton
 
-open NFA DFA
+open NFA DFA εNFA
 
-def Q : Finset (Fin 2) := {0,1}
-def σ : Finset (Fin 2) := {0,1}
+def Q₁ : Finset (Fin 2) := {0,1}
+def σ₁ : Finset (Fin 2) := {0,1}
 
-def δ₁ : Q → σ → Finset Q
+def δ₁ : Q₁ → σ₁ → Finset Q₁
   | ⟨0, _⟩ , ⟨1,_⟩ => {⟨1,by simp⟩}
   | ⟨0, _⟩ , ⟨0,_⟩ => {⟨0,by simp⟩}
   | ⟨1, _⟩ , ⟨1,_⟩ => {⟨1,by simp⟩}
   | ⟨1, _⟩ , ⟨0,_⟩ => {⟨0,by simp⟩}
 
-def nfa₁ : @NFA (Fin 2) (Fin 2) := {qs := Q, init := ⟨0,by simp⟩, fs := {⟨1,by simp⟩} , δ := δ₁}
+def nfa₁ : NFA Q₁ σ₁ := {init := ⟨0,by simp⟩, fs := {⟨1,by simp⟩} , δ := δ₁}
 
-def w₁ : word σ := []
-def w₂ : word σ := [⟨1, by simp⟩ , ⟨0, by simp⟩]
-def w₃ : word σ := [⟨0, by simp⟩ , ⟨1, by simp⟩]
+def w₁₁ : word σ₁ := []
+def w₁₂ : word σ₁ := [⟨1, by simp⟩ , ⟨0, by simp⟩]
+def w₁₃ : word σ₁ := [⟨0, by simp⟩ , ⟨1, by simp⟩]
 
-#eval nfa_accepts nfa₁ w₁
-#eval nfa_accepts nfa₁ w₂
-#eval nfa_accepts nfa₁ w₃
+#eval nfa_accepts nfa₁ w₁₁
+#eval nfa_accepts nfa₁ w₁₂
+#eval nfa_accepts nfa₁ w₁₃
 
-#eval dfa_accepts (ToDFA.nfa_to_dfa nfa₁) w₁
-#eval dfa_accepts (ToDFA.nfa_to_dfa nfa₁) w₂
-#eval dfa_accepts (ToDFA.nfa_to_dfa nfa₁) w₃
+#eval dfa_accepts (ToDFA.nfa_to_dfa nfa₁) w₁₁
+#eval dfa_accepts (ToDFA.nfa_to_dfa nfa₁) w₁₂
+#eval dfa_accepts (ToDFA.nfa_to_dfa nfa₁) w₁₃
 
-#eval nfa_accepts (ToNFA.dfa_to_nfa (ToDFA.nfa_to_dfa nfa₁)) w₁
-#eval nfa_accepts (ToNFA.dfa_to_nfa (ToDFA.nfa_to_dfa nfa₁)) w₂
-#eval nfa_accepts (ToNFA.dfa_to_nfa (ToDFA.nfa_to_dfa nfa₁)) w₃
+#eval nfa_accepts (ToNFA.dfa_to_nfa (ToDFA.nfa_to_dfa nfa₁)) w₁₁
+#eval nfa_accepts (ToNFA.dfa_to_nfa (ToDFA.nfa_to_dfa nfa₁)) w₁₂
+#eval nfa_accepts (ToNFA.dfa_to_nfa (ToDFA.nfa_to_dfa nfa₁)) w₁₃
+
+
+def Q₂ : Finset (Fin 4) := {0,1,2,3}
+def σ₂ : Finset (Fin 3) := {0,1,2}
+
+def δ₂ : Q₂ → Option σ₂ → Finset Q₂
+  | ⟨0, _⟩ , some ⟨0,_⟩ => {⟨0,by simp⟩}
+  | ⟨0, _⟩ , none => {⟨1,by simp⟩}
+  | ⟨1, _⟩ , some ⟨1,_⟩ => {⟨1,by simp⟩}
+  | ⟨1, _⟩ , none => {⟨2,by simp⟩}
+  | ⟨2, _⟩ , some ⟨2,_⟩ => {⟨3,by simp⟩}
+  | _ , _ => ∅
+
+-- accepts any number of 0s followed by any number of 1s followed by exactly one 2
+def εnfa₂ : εNFA σ₂ Q₂ := {init := ⟨0,by simp⟩, fs := {⟨3,by simp⟩}, δ := δ₂}
+
+
+def w₂₁ : word σ₂ := []
+def w₂₂ : word σ₂ := [⟨0,by simp⟩]
+def w₂₃ : word σ₂ := [⟨1,by simp⟩]
+def w₂₄ : word σ₂ := [⟨2,by simp⟩]
+def w₂₅ : word σ₂ := [⟨0,by simp⟩, ⟨0,by simp⟩, ⟨0,by simp⟩, ⟨1,by simp⟩, ⟨2,by simp⟩]
+def w₂₆ : word σ₂ := [⟨0,by simp⟩, ⟨0,by simp⟩, ⟨0,by simp⟩, ⟨1,by simp⟩]
+
+#eval εnfa_accepts εnfa₂ w₂₁
+#eval εnfa_accepts εnfa₂ w₂₂
+#eval εnfa_accepts εnfa₂ w₂₃
+#eval εnfa_accepts εnfa₂ w₂₄
+#eval εnfa_accepts εnfa₂ w₂₅
+#eval εnfa_accepts εnfa₂ w₂₆
+
+#eval nfa_accepts (εnfa_to_nfa εnfa₂) w₂₁
+#eval nfa_accepts (εnfa_to_nfa εnfa₂) w₂₂
+#eval nfa_accepts (εnfa_to_nfa εnfa₂) w₂₃
+#eval nfa_accepts (εnfa_to_nfa εnfa₂) w₂₄
+#eval nfa_accepts (εnfa_to_nfa εnfa₂) w₂₅
+#eval nfa_accepts (εnfa_to_nfa εnfa₂) w₂₆
+
+
